AwsCryptographicMaterialProviders/dafny/AwsCryptographyKeyStoreAdmin/src/InitializeMutation.dfy
@@ -170,6 +170,19 @@ module {:options "/functionSyntax:4" } InternalInitializeMutation {
     }
 
     if (readItems.MutationCommitment.Some?) {
+      :- Need(
+        StateStrucs.ValidCommitment?(readItems.MutationCommitment.value),
+        Types.AwsCryptographyKeyStore(
+          // We decided that Storage would not care about the Byte Structure of MUTATION_COMMITMENT's attributes.
+          // But I think a Storage Exception makes sense for a corrupted item.
+          AwsCryptographyKeyStore := KeyStoreTypes.KeyStorageException(
+            message := "Mutation Commitment read from Storage is invalid or corrupted."
+            + " Recommend auditing the Branch Key's items for tampering."
+            + " Recommend auditing access to the storage."
+            + " To successfully start a new mutation, delete the Mutation Commitment."
+            + " But know that the new mutation will fail if any corrupt items are encountered."
+            + "\nBranch Key ID: " + input.Identifier + ";"
+            + " Mutation Commitment UUID: " + readItems.MutationCommitment.value.UUID)));
       resumeMutation? :- CommitmentAndInputMatch(
         internalInput := input,
         commitment := readItems.MutationCommitment.value);
